Updated creusot

creusot_sandbox/mlcfg/creusot_sandbox/creusot_sandbox_CreusotSandbox_UnionFind_Impl1_LemmaBelongUnique_Impl_lemma_belong_uniqueqtvc_1.v
@@ -20,25 +20,37 @@ Definition contents {a:Type} {a_WT:WhyType a} (v:ref a) : a :=
   | ref'mk x => x
   end.
 
-(* Why3 assumption *)
-Inductive borrowed (a:Type) :=
-  | borrowed'mk : a -> a -> borrowed a.
-Axiom borrowed_WhyType : forall (a:Type) {a_WT:WhyType a},
-  WhyType (borrowed a).
-Existing Instance borrowed_WhyType.
-Arguments borrowed'mk {a}.
+Axiom uint64 : Type.
+Parameter uint64_WhyType : WhyType uint64.
+Existing Instance uint64_WhyType.
+
+Parameter uint64'int: uint64 -> Numbers.BinNums.Z.
+
+Axiom uint64'axiom :
+  forall (i:uint64),
+  (0%Z <= (uint64'int i))%Z /\ ((uint64'int i) <= 18446744073709551615%Z)%Z.
 
 (* Why3 assumption *)
-Definition current {a:Type} {a_WT:WhyType a} (v:borrowed a) : a :=
-  match v with
-  | borrowed'mk x x1 => x
-  end.
+Definition uint64'eq (a:uint64) (b:uint64) : Prop :=
+  ((uint64'int a) = (uint64'int b)).
+
+Axiom uint64'inj : forall (a:uint64) (b:uint64), uint64'eq a b -> (a = b).
 
 (* Why3 assumption *)
-Definition final {a:Type} {a_WT:WhyType a} (v:borrowed a) : a :=
-  match v with
-  | borrowed'mk x x1 => x1
-  end.
+Definition in_bounds (n:Numbers.BinNums.Z) : Prop :=
+  (0%Z <= n)%Z /\ (n <= 18446744073709551615%Z)%Z.
+
+Axiom to_int_in_bounds : forall (n:uint64), in_bounds (uint64'int n).
+
+Axiom extensionality :
+  forall (x:uint64) (y:uint64), ((uint64'int x) = (uint64'int y)) -> (x = y).
+
+Parameter zero_unsigned: uint64.
+
+Axiom zero_unsigned_is_zero : ((uint64'int zero_unsigned) = 0%Z).
+
+(* Why3 assumption *)
+Definition usize := uint64.
 
 Axiom seq : forall (a:Type), Type.
 Parameter seq_WhyType : forall (a:Type) {a_WT:WhyType a}, WhyType (seq a).
@@ -56,26 +68,32 @@ Parameter get:
 Parameter infix_eqeq:
   forall {a:Type} {a_WT:WhyType a}, seq a -> seq a -> Prop.
 
-Axiom infix_eqeq'spec :
+Axiom infix_eqeq'spec'0 :
   forall {a:Type} {a_WT:WhyType a},
   forall (s1:seq a) (s2:seq a),
-  (infix_eqeq s1 s2 <->
-   ((length s1) = (length s2)) /\
-   (forall (i:Numbers.BinNums.Z), (0%Z <= i)%Z /\ (i < (length s1))%Z ->
-    ((get s1 i) = (get s2 i)))) /\
-  (infix_eqeq s1 s2 -> (s1 = s2)).
+  infix_eqeq s1 s2 <->
+  ((length s1) = (length s2)) /\
+  (forall (i:Numbers.BinNums.Z), (0%Z <= i)%Z /\ (i < (length s1))%Z ->
+   ((get s1 i) = (get s2 i))).
+
+Axiom infix_eqeq'spec :
+  forall {a:Type} {a_WT:WhyType a},
+  forall (s1:seq a) (s2:seq a), infix_eqeq s1 s2 -> (s1 = s2).
 
 Parameter create:
   forall {a:Type} {a_WT:WhyType a}, Numbers.BinNums.Z ->
   (Numbers.BinNums.Z -> a) -> seq a.
 
+Axiom create'spec'0 :
+  forall {a:Type} {a_WT:WhyType a},
+  forall (len:Numbers.BinNums.Z) (f:Numbers.BinNums.Z -> a),
+  (0%Z <= len)%Z -> ((length (create len f)) = len).
+
 Axiom create'spec :
   forall {a:Type} {a_WT:WhyType a},
   forall (len:Numbers.BinNums.Z) (f:Numbers.BinNums.Z -> a),
-  (0%Z <= len)%Z ->
-  ((length (create len f)) = len) /\
-  (forall (i:Numbers.BinNums.Z), (0%Z <= i)%Z /\ (i < len)%Z ->
-   ((get (create len f) i) = (f i))).
+  (0%Z <= len)%Z -> forall (i:Numbers.BinNums.Z),
+  (0%Z <= i)%Z /\ (i < len)%Z -> ((get (create len f) i) = (f i)).
 
 Parameter empty: forall {a:Type} {a_WT:WhyType a}, seq a.
 
@@ -101,15 +119,22 @@ Axiom set'def :
   (0%Z <= i)%Z /\ (i < (length s))%Z ->
   ((set s i v) = (create (length s) (result s i v))).
 
+Axiom set'spec'1 :
+  forall {a:Type} {a_WT:WhyType a},
+  forall (s:seq a) (i:Numbers.BinNums.Z) (v:a),
+  (0%Z <= i)%Z /\ (i < (length s))%Z -> ((length (set s i v)) = (length s)).
+
+Axiom set'spec'0 :
+  forall {a:Type} {a_WT:WhyType a},
+  forall (s:seq a) (i:Numbers.BinNums.Z) (v:a),
+  (0%Z <= i)%Z /\ (i < (length s))%Z -> ((get (set s i v) i) = v).
+
 Axiom set'spec :
   forall {a:Type} {a_WT:WhyType a},
   forall (s:seq a) (i:Numbers.BinNums.Z) (v:a),
-  (0%Z <= i)%Z /\ (i < (length s))%Z ->
-  ((length (set s i v)) = (length s)) /\
-  ((get (set s i v) i) = v) /\
-  (forall (j:Numbers.BinNums.Z),
-   ((0%Z <= j)%Z /\ (j < (length s))%Z) /\ ~ (j = i) ->
-   ((get (set s i v) j) = (get s j))).
+  (0%Z <= i)%Z /\ (i < (length s))%Z -> forall (j:Numbers.BinNums.Z),
+  ((0%Z <= j)%Z /\ (j < (length s))%Z) /\ ~ (j = i) ->
+  ((get (set s i v) j) = (get s j)).
 
 Parameter mixfix_lblsmnrb:
   forall {a:Type} {a_WT:WhyType a}, seq a -> Numbers.BinNums.Z -> a -> seq a.
@@ -124,10 +149,13 @@ Axiom mixfix_lblsmnrb'def :
 Definition singleton {a:Type} {a_WT:WhyType a} (v:a) : seq a :=
   create 1%Z (fun (us:Numbers.BinNums.Z) => v).
 
+Axiom singleton'spec'0 :
+  forall {a:Type} {a_WT:WhyType a},
+  forall (v:a), ((length (singleton v)) = 1%Z).
+
 Axiom singleton'spec :
   forall {a:Type} {a_WT:WhyType a},
-  forall (v:a),
-  ((length (singleton v)) = 1%Z) /\ ((get (singleton v) 0%Z) = v).
+  forall (v:a), ((get (singleton v) 0%Z) = v).
 
 Parameter result1:
   forall {a:Type} {a_WT:WhyType a}, a -> seq a -> Numbers.BinNums.Z -> a.
@@ -142,13 +170,19 @@ Axiom result'def1 :
 Definition cons {a:Type} {a_WT:WhyType a} (x:a) (s:seq a) : seq a :=
   create (1%Z + (length s))%Z (result1 x s).
 
+Axiom cons'spec'1 :
+  forall {a:Type} {a_WT:WhyType a},
+  forall (x:a) (s:seq a), ((length (cons x s)) = (1%Z + (length s))%Z).
+
+Axiom cons'spec'0 :
+  forall {a:Type} {a_WT:WhyType a},
+  forall (x:a) (s:seq a), ((get (cons x s) 0%Z) = x).
+
 Axiom cons'spec :
   forall {a:Type} {a_WT:WhyType a},
-  forall (x:a) (s:seq a),
-  ((length (cons x s)) = (1%Z + (length s))%Z) /\
-  ((get (cons x s) 0%Z) = x) /\
-  (forall (i:Numbers.BinNums.Z), (0%Z < i)%Z /\ (i <= (length s))%Z ->
-   ((get (cons x s) i) = (get s (i - 1%Z)%Z))).
+  forall (x:a) (s:seq a), forall (i:Numbers.BinNums.Z),
+  (0%Z < i)%Z /\ (i <= (length s))%Z ->
+  ((get (cons x s) i) = (get s (i - 1%Z)%Z)).
 
 Parameter result2:
   forall {a:Type} {a_WT:WhyType a}, seq a -> a -> Numbers.BinNums.Z -> a.
@@ -163,13 +197,18 @@ Axiom result'def2 :
 Definition snoc {a:Type} {a_WT:WhyType a} (s:seq a) (x:a) : seq a :=
   create (1%Z + (length s))%Z (result2 s x).
 
+Axiom snoc'spec'1 :
+  forall {a:Type} {a_WT:WhyType a},
+  forall (s:seq a) (x:a), ((length (snoc s x)) = (1%Z + (length s))%Z).
+
+Axiom snoc'spec'0 :
+  forall {a:Type} {a_WT:WhyType a},
+  forall (s:seq a) (x:a), ((get (snoc s x) (length s)) = x).
+
 Axiom snoc'spec :
   forall {a:Type} {a_WT:WhyType a},
-  forall (s:seq a) (x:a),
-  ((length (snoc s x)) = (1%Z + (length s))%Z) /\
-  ((get (snoc s x) (length s)) = x) /\
-  (forall (i:Numbers.BinNums.Z), (0%Z <= i)%Z /\ (i < (length s))%Z ->
-   ((get (snoc s x) i) = (get s i))).
+  forall (s:seq a) (x:a), forall (i:Numbers.BinNums.Z),
+  (0%Z <= i)%Z /\ (i < (length s))%Z -> ((get (snoc s x) i) = (get s i)).
 
 Parameter mixfix_lbdtdtrb:
   forall {a:Type} {a_WT:WhyType a}, seq a -> Numbers.BinNums.Z ->
@@ -182,13 +221,18 @@ Axiom mixfix_lbdtdtrb'def :
   ((mixfix_lbdtdtrb s i j) =
    (create (j - i)%Z (fun (k:Numbers.BinNums.Z) => get s (i + k)%Z))).
 
+Axiom mixfix_lbdtdtrb'spec'0 :
+  forall {a:Type} {a_WT:WhyType a},
+  forall (s:seq a) (i:Numbers.BinNums.Z) (j:Numbers.BinNums.Z),
+  (0%Z <= i)%Z /\ (i <= j)%Z /\ (j <= (length s))%Z ->
+  ((length (mixfix_lbdtdtrb s i j)) = (j - i)%Z).
+
 Axiom mixfix_lbdtdtrb'spec :
   forall {a:Type} {a_WT:WhyType a},
   forall (s:seq a) (i:Numbers.BinNums.Z) (j:Numbers.BinNums.Z),
   (0%Z <= i)%Z /\ (i <= j)%Z /\ (j <= (length s))%Z ->
-  ((length (mixfix_lbdtdtrb s i j)) = (j - i)%Z) /\
-  (forall (k:Numbers.BinNums.Z), (0%Z <= k)%Z /\ (k < (j - i)%Z)%Z ->
-   ((get (mixfix_lbdtdtrb s i j) k) = (get s (i + k)%Z))).
+  forall (k:Numbers.BinNums.Z), (0%Z <= k)%Z /\ (k < (j - i)%Z)%Z ->
+  ((get (mixfix_lbdtdtrb s i j) k) = (get s (i + k)%Z)).
 
 Parameter mixfix_lb_dtdtrb:
   forall {a:Type} {a_WT:WhyType a}, seq a -> Numbers.BinNums.Z -> seq a.
@@ -222,41 +266,22 @@ Axiom result'def3 :
 Definition infix_plpl {a:Type} {a_WT:WhyType a} (s1:seq a) (s2:seq a) : seq a :=
   let l := length s1 in create (l + (length s2))%Z (result3 s1 s2 l).
 
-Axiom infix_plpl'spec :
+Axiom infix_plpl'spec'1 :
   forall {a:Type} {a_WT:WhyType a},
   forall (s1:seq a) (s2:seq a),
-  ((length (infix_plpl s1 s2)) = ((length s1) + (length s2))%Z) /\
-  (forall (i:Numbers.BinNums.Z), (0%Z <= i)%Z /\ (i < (length s1))%Z ->
-   ((get (infix_plpl s1 s2) i) = (get s1 i))) /\
-  (forall (i:Numbers.BinNums.Z),
-   ((length s1) <= i)%Z /\ (i < (length (infix_plpl s1 s2)))%Z ->
-   ((get (infix_plpl s1 s2) i) = (get s2 (i - (length s1))%Z))).
+  ((length (infix_plpl s1 s2)) = ((length s1) + (length s2))%Z).
 
-Axiom uint64 : Type.
-Parameter uint64_WhyType : WhyType uint64.
-Existing Instance uint64_WhyType.
+Axiom infix_plpl'spec'0 :
+  forall {a:Type} {a_WT:WhyType a},
+  forall (s1:seq a) (s2:seq a), forall (i:Numbers.BinNums.Z),
+  (0%Z <= i)%Z /\ (i < (length s1))%Z ->
+  ((get (infix_plpl s1 s2) i) = (get s1 i)).
 
-Parameter uint64'int: uint64 -> Numbers.BinNums.Z.
-
-Axiom uint64'axiom :
-  forall (i:uint64),
-  (0%Z <= (uint64'int i))%Z /\ ((uint64'int i) <= 18446744073709551615%Z)%Z.
-
-(* Why3 assumption *)
-Definition in_bounds (n:Numbers.BinNums.Z) : Prop :=
-  (0%Z <= n)%Z /\ (n <= 18446744073709551615%Z)%Z.
-
-Axiom to_int_in_bounds : forall (n:uint64), in_bounds (uint64'int n).
-
-Axiom extensionality :
-  forall (x:uint64) (y:uint64), ((uint64'int x) = (uint64'int y)) -> (x = y).
-
-Parameter zero_unsigned: uint64.
-
-Axiom zero_unsigned_is_zero : ((uint64'int zero_unsigned) = 0%Z).
-
-(* Why3 assumption *)
-Definition usize := uint64.
+Axiom infix_plpl'spec :
+  forall {a:Type} {a_WT:WhyType a},
+  forall (s1:seq a) (s2:seq a), forall (i:Numbers.BinNums.Z),
+  ((length s1) <= i)%Z /\ (i < (length (infix_plpl s1 s2)))%Z ->
+  ((get (infix_plpl s1 s2) i) = (get s2 (i - (length s1))%Z)).
 
 (* Why3 assumption *)
 Inductive t_unionfindmodel :=
@@ -271,88 +296,124 @@ Definition unionfindmodel_parent (self:t_unionfindmodel) : seq uint64 :=
   end.
 
 (* Why3 assumption *)
-Definition in_range (self:t_unionfindmodel) (i:Numbers.BinNums.Z) : Prop :=
-  (0%Z <= i)%Z /\ (i < (length (unionfindmodel_parent self)))%Z.
+Inductive borrowed
+  (a:Type) :=
+  | borrowed'mk : a -> a -> Numbers.BinNums.Z -> borrowed a.
+Axiom borrowed_WhyType : forall (a:Type) {a_WT:WhyType a},
+  WhyType (borrowed a).
+Existing Instance borrowed_WhyType.
+Arguments borrowed'mk {a}.
 
 (* Why3 assumption *)
-Definition parent (self:t_unionfindmodel) (i:Numbers.BinNums.Z) :
+Definition current {a:Type} {a_WT:WhyType a} (v:borrowed a) : a :=
+  match v with
+  | borrowed'mk x x1 x2 => x
+  end.
+
+(* Why3 assumption *)
+Definition final {a:Type} {a_WT:WhyType a} (v:borrowed a) : a :=
+  match v with
+  | borrowed'mk x x1 x2 => x1
+  end.
+
+(* Why3 assumption *)
+Definition id {a:Type} {a_WT:WhyType a} (v:borrowed a) : Numbers.BinNums.Z :=
+  match v with
+  | borrowed'mk x x1 x2 => x2
+  end.
+
+Parameter inherit_id:
+  Numbers.BinNums.Z -> Numbers.BinNums.Z -> Numbers.BinNums.Z.
+
+(* Why3 assumption *)
+Definition parent0 (self:t_unionfindmodel) (i:Numbers.BinNums.Z) :
     Numbers.BinNums.Z :=
   uint64'int (get (unionfindmodel_parent self) i).
 
-Parameter reach:
+Parameter reach0:
   t_unionfindmodel -> Numbers.BinNums.Z -> Numbers.BinNums.Z ->
   Numbers.BinNums.Z -> Prop.
 
-Axiom def :
+Axiom reach0_def :
   forall (self:t_unionfindmodel) (src:Numbers.BinNums.Z)
     (dst:Numbers.BinNums.Z) (len:Numbers.BinNums.Z),
-  (reach self src dst len ->
+  (reach0 self src dst len ->
    ~ (len < 0%Z)%Z /\
-   (~ (len < 0%Z)%Z ->
-    ((len = 0%Z) -> (src = dst)) /\
-    (~ (len = 0%Z) ->
-     ~ (src = dst) /\ reach self (parent self src) dst (len - 1%Z)%Z))) /\
+   ((len = 0%Z) -> (src = dst)) /\
+   (~ (len = 0%Z) ->
+    ~ (src = dst) /\ reach0 self (parent0 self src) dst (len - 1%Z)%Z)) /\
   (~ (len < 0%Z)%Z /\
    ((len = 0%Z) /\ (src = dst) \/
     ~ (len = 0%Z) /\
-    ~ (src = dst) /\ reach self (parent self src) dst (len - 1%Z)%Z) ->
-   reach self src dst len).
+    ~ (src = dst) /\ reach0 self (parent0 self src) dst (len - 1%Z)%Z) ->
+   reach0 self src dst len).
 
-Axiom reach_spec : True.
-
-(* Why3 assumption *)
-Definition is_root (self:t_unionfindmodel) (i:Numbers.BinNums.Z) : Prop :=
-  in_range self i /\ ((parent self i) = i).
-
-Axiom lemma_reach_iff_spec :
+Axiom lemma_reach_iff0_spec :
   forall (self:t_unionfindmodel), forall (len:Numbers.BinNums.Z),
   forall (dst:Numbers.BinNums.Z), forall (src:Numbers.BinNums.Z),
-  reach self src dst len <->
+  reach0 self src dst len <->
   (src = dst) /\ (len = 0%Z) \/
   ~ (src = dst) /\
-  (0%Z < len)%Z /\ reach self (parent self src) dst (len - 1%Z)%Z.
+  (0%Z < len)%Z /\ reach0 self (parent0 self src) dst (len - 1%Z)%Z.
 
 (* Why3 assumption *)
-Definition belong (self:t_unionfindmodel) (i:Numbers.BinNums.Z)
+Definition in_range0 (self:t_unionfindmodel) (i:Numbers.BinNums.Z) : Prop :=
+  (0%Z <= i)%Z /\ (i < (length (unionfindmodel_parent self)))%Z.
+
+(* Why3 assumption *)
+Definition is_root0 (self:t_unionfindmodel) (i:Numbers.BinNums.Z) : Prop :=
+  in_range0 self i /\ ((parent0 self i) = i).
+
+(* Why3 assumption *)
+Definition belong0 (self:t_unionfindmodel) (i:Numbers.BinNums.Z)
     (root:Numbers.BinNums.Z) : Prop :=
-  is_root self root /\ (exists len:Numbers.BinNums.Z, reach self i root len).
+  is_root0 self root /\
+  (exists len:Numbers.BinNums.Z, reach0 self i root len).
+
+Parameter self: t_unionfindmodel.
+
+Parameter lemma_belong_unique: t_unionfindmodel -> Init.Datatypes.unit.
 
 Lemma root_reachable : forall uf i j n,
-    is_root uf i -> reach uf i j n -> j = i.
+    is_root0 uf i -> reach0 uf i j n -> j = i.
 Proof.
   intros uf i j n [_ Hparent] Hreach.
   induction n as [n IH] using (well_founded_induction (Z.lt_wf 0)).
-  rewrite lemma_reach_iff_spec in Hreach.
+  rewrite lemma_reach_iff0_spec in Hreach.
   destruct Hreach as [|(Hne & Hpos & Hreach)]; [intuition| ].
   rewrite Hparent in Hreach.
   apply IH in Hreach; auto with zarith.
 Qed.
 
+
 (* Why3 goal *)
-Theorem lemma_belong_unique'vc :
-  forall (self:seq uint64),
-  let self1 := C_UnionFindModel self in
+Theorem vc_lemma_belong_unique :
+  (forall (len:Numbers.BinNums.Z), forall (dst:Numbers.BinNums.Z),
+   forall (src:Numbers.BinNums.Z),
+   reach0 self src dst len <->
+   (src = dst) /\ (len = 0%Z) \/
+   ~ (src = dst) /\
+   (0%Z < len)%Z /\ reach0 self (parent0 self src) dst (len - 1%Z)%Z) ->
   forall (r2:Numbers.BinNums.Z), forall (r1:Numbers.BinNums.Z),
-  forall (i:Numbers.BinNums.Z), belong self1 i r1 -> belong self1 i r2 ->
+  forall (i:Numbers.BinNums.Z), belong0 self i r1 -> belong0 self i r2 ->
   (r1 = r2).
-(* Why3 intros self self1 r2 r1 i h1 h2. *)
 Proof.
-  intros self_parent self.
+  intros _.
   intros r2 r1 i (Hroot1 & len1 & Hreach1) (Hroot2 & len2 & Hreach2).
   revert i len2 Hreach1 Hreach2.
   induction len1 as [len1 IH] using (well_founded_induction (Z.lt_wf 0)).
   intros i len2 Hreach1 Hreach2.
-  rewrite lemma_reach_iff_spec in Hreach1.
+  rewrite lemma_reach_iff0_spec in Hreach1.
   destruct Hreach1 as [Hreach1 | Hreach1].
   - destruct Hreach1. subst.
     apply root_reachable in Hreach2; auto.
   - destruct Hreach1 as (Hne & Hpos & Hreach).
-    rewrite lemma_reach_iff_spec in Hreach2.
+    rewrite lemma_reach_iff0_spec in Hreach2.
     destruct Hreach2 as [Hreach2 | Hreach2].
     + destruct Hreach2. subst.
       rewrite (proj2 Hroot2) in *.
       eauto using root_reachable.
     + destruct Hreach2 as (_ & _ & Hreach2).
       eapply IH in Hreach; eauto with zarith.
-Qed.
 
+Qed.
