creusot_sandbox/mlcfg/creusot_sandbox/creusot_sandbox_CreusotSandbox_UnionFind_Impl1_LemmaUpdateBelongUpdated_Impl_lemma_update_belong_updatedqtvc_1.v
@@ -31,6 +31,12 @@ Axiom uint64'axiom :
   (0%Z <= (uint64'int i))%Z /\ ((uint64'int i) <= 18446744073709551615%Z)%Z.
 
 (* Why3 assumption *)
+Definition uint64'eq (a:uint64) (b:uint64) : Prop :=
+  ((uint64'int a) = (uint64'int b)).
+
+Axiom uint64'inj : forall (a:uint64) (b:uint64), uint64'eq a b -> (a = b).
+
+(* Why3 assumption *)
 Definition in_bounds (n:Numbers.BinNums.Z) : Prop :=
   (0%Z <= n)%Z /\ (n <= 18446744073709551615%Z)%Z.
 
@@ -42,26 +48,6 @@ Axiom extensionality :
 Parameter zero_unsigned: uint64.
 
 Axiom zero_unsigned_is_zero : ((uint64'int zero_unsigned) = 0%Z).
-
-(* Why3 assumption *)
-Inductive borrowed (a:Type) :=
-  | borrowed'mk : a -> a -> borrowed a.
-Axiom borrowed_WhyType : forall (a:Type) {a_WT:WhyType a},
-  WhyType (borrowed a).
-Existing Instance borrowed_WhyType.
-Arguments borrowed'mk {a}.
-
-(* Why3 assumption *)
-Definition current {a:Type} {a_WT:WhyType a} (v:borrowed a) : a :=
-  match v with
-  | borrowed'mk x x1 => x
-  end.
-
-(* Why3 assumption *)
-Definition final {a:Type} {a_WT:WhyType a} (v:borrowed a) : a :=
-  match v with
-  | borrowed'mk x x1 => x1
-  end.
 
 (* Why3 assumption *)
 Definition usize := uint64.
@@ -82,26 +68,32 @@ Parameter get:
 Parameter infix_eqeq:
   forall {a:Type} {a_WT:WhyType a}, seq a -> seq a -> Prop.
 
-Axiom infix_eqeq'spec :
+Axiom infix_eqeq'spec'0 :
   forall {a:Type} {a_WT:WhyType a},
   forall (s1:seq a) (s2:seq a),
-  (infix_eqeq s1 s2 <->
-   ((length s1) = (length s2)) /\
-   (forall (i:Numbers.BinNums.Z), (0%Z <= i)%Z /\ (i < (length s1))%Z ->
-    ((get s1 i) = (get s2 i)))) /\
-  (infix_eqeq s1 s2 -> (s1 = s2)).
+  infix_eqeq s1 s2 <->
+  ((length s1) = (length s2)) /\
+  (forall (i:Numbers.BinNums.Z), (0%Z <= i)%Z /\ (i < (length s1))%Z ->
+   ((get s1 i) = (get s2 i))).
+
+Axiom infix_eqeq'spec :
+  forall {a:Type} {a_WT:WhyType a},
+  forall (s1:seq a) (s2:seq a), infix_eqeq s1 s2 -> (s1 = s2).
 
 Parameter create:
   forall {a:Type} {a_WT:WhyType a}, Numbers.BinNums.Z ->
   (Numbers.BinNums.Z -> a) -> seq a.
 
+Axiom create'spec'0 :
+  forall {a:Type} {a_WT:WhyType a},
+  forall (len:Numbers.BinNums.Z) (f:Numbers.BinNums.Z -> a),
+  (0%Z <= len)%Z -> ((length (create len f)) = len).
+
 Axiom create'spec :
   forall {a:Type} {a_WT:WhyType a},
   forall (len:Numbers.BinNums.Z) (f:Numbers.BinNums.Z -> a),
-  (0%Z <= len)%Z ->
-  ((length (create len f)) = len) /\
-  (forall (i:Numbers.BinNums.Z), (0%Z <= i)%Z /\ (i < len)%Z ->
-   ((get (create len f) i) = (f i))).
+  (0%Z <= len)%Z -> forall (i:Numbers.BinNums.Z),
+  (0%Z <= i)%Z /\ (i < len)%Z -> ((get (create len f) i) = (f i)).
 
 Parameter empty: forall {a:Type} {a_WT:WhyType a}, seq a.
 
@@ -127,15 +119,22 @@ Axiom set'def :
   (0%Z <= i)%Z /\ (i < (length s))%Z ->
   ((set s i v) = (create (length s) (result s i v))).
 
+Axiom set'spec'1 :
+  forall {a:Type} {a_WT:WhyType a},
+  forall (s:seq a) (i:Numbers.BinNums.Z) (v:a),
+  (0%Z <= i)%Z /\ (i < (length s))%Z -> ((length (set s i v)) = (length s)).
+
+Axiom set'spec'0 :
+  forall {a:Type} {a_WT:WhyType a},
+  forall (s:seq a) (i:Numbers.BinNums.Z) (v:a),
+  (0%Z <= i)%Z /\ (i < (length s))%Z -> ((get (set s i v) i) = v).
+
 Axiom set'spec :
   forall {a:Type} {a_WT:WhyType a},
   forall (s:seq a) (i:Numbers.BinNums.Z) (v:a),
-  (0%Z <= i)%Z /\ (i < (length s))%Z ->
-  ((length (set s i v)) = (length s)) /\
-  ((get (set s i v) i) = v) /\
-  (forall (j:Numbers.BinNums.Z),
-   ((0%Z <= j)%Z /\ (j < (length s))%Z) /\ ~ (j = i) ->
-   ((get (set s i v) j) = (get s j))).
+  (0%Z <= i)%Z /\ (i < (length s))%Z -> forall (j:Numbers.BinNums.Z),
+  ((0%Z <= j)%Z /\ (j < (length s))%Z) /\ ~ (j = i) ->
+  ((get (set s i v) j) = (get s j)).
 
 Parameter mixfix_lblsmnrb:
   forall {a:Type} {a_WT:WhyType a}, seq a -> Numbers.BinNums.Z -> a -> seq a.
@@ -150,10 +149,13 @@ Axiom mixfix_lblsmnrb'def :
 Definition singleton {a:Type} {a_WT:WhyType a} (v:a) : seq a :=
   create 1%Z (fun (us:Numbers.BinNums.Z) => v).
 
+Axiom singleton'spec'0 :
+  forall {a:Type} {a_WT:WhyType a},
+  forall (v:a), ((length (singleton v)) = 1%Z).
+
 Axiom singleton'spec :
   forall {a:Type} {a_WT:WhyType a},
-  forall (v:a),
-  ((length (singleton v)) = 1%Z) /\ ((get (singleton v) 0%Z) = v).
+  forall (v:a), ((get (singleton v) 0%Z) = v).
 
 Parameter result1:
   forall {a:Type} {a_WT:WhyType a}, a -> seq a -> Numbers.BinNums.Z -> a.
@@ -168,13 +170,19 @@ Axiom result'def1 :
 Definition cons {a:Type} {a_WT:WhyType a} (x:a) (s:seq a) : seq a :=
   create (1%Z + (length s))%Z (result1 x s).
 
+Axiom cons'spec'1 :
+  forall {a:Type} {a_WT:WhyType a},
+  forall (x:a) (s:seq a), ((length (cons x s)) = (1%Z + (length s))%Z).
+
+Axiom cons'spec'0 :
+  forall {a:Type} {a_WT:WhyType a},
+  forall (x:a) (s:seq a), ((get (cons x s) 0%Z) = x).
+
 Axiom cons'spec :
   forall {a:Type} {a_WT:WhyType a},
-  forall (x:a) (s:seq a),
-  ((length (cons x s)) = (1%Z + (length s))%Z) /\
-  ((get (cons x s) 0%Z) = x) /\
-  (forall (i:Numbers.BinNums.Z), (0%Z < i)%Z /\ (i <= (length s))%Z ->
-   ((get (cons x s) i) = (get s (i - 1%Z)%Z))).
+  forall (x:a) (s:seq a), forall (i:Numbers.BinNums.Z),
+  (0%Z < i)%Z /\ (i <= (length s))%Z ->
+  ((get (cons x s) i) = (get s (i - 1%Z)%Z)).
 
 Parameter result2:
   forall {a:Type} {a_WT:WhyType a}, seq a -> a -> Numbers.BinNums.Z -> a.
@@ -189,13 +197,18 @@ Axiom result'def2 :
 Definition snoc {a:Type} {a_WT:WhyType a} (s:seq a) (x:a) : seq a :=
   create (1%Z + (length s))%Z (result2 s x).
 
+Axiom snoc'spec'1 :
+  forall {a:Type} {a_WT:WhyType a},
+  forall (s:seq a) (x:a), ((length (snoc s x)) = (1%Z + (length s))%Z).
+
+Axiom snoc'spec'0 :
+  forall {a:Type} {a_WT:WhyType a},
+  forall (s:seq a) (x:a), ((get (snoc s x) (length s)) = x).
+
 Axiom snoc'spec :
   forall {a:Type} {a_WT:WhyType a},
-  forall (s:seq a) (x:a),
-  ((length (snoc s x)) = (1%Z + (length s))%Z) /\
-  ((get (snoc s x) (length s)) = x) /\
-  (forall (i:Numbers.BinNums.Z), (0%Z <= i)%Z /\ (i < (length s))%Z ->
-   ((get (snoc s x) i) = (get s i))).
+  forall (s:seq a) (x:a), forall (i:Numbers.BinNums.Z),
+  (0%Z <= i)%Z /\ (i < (length s))%Z -> ((get (snoc s x) i) = (get s i)).
 
 Parameter mixfix_lbdtdtrb:
   forall {a:Type} {a_WT:WhyType a}, seq a -> Numbers.BinNums.Z ->
@@ -208,13 +221,18 @@ Axiom mixfix_lbdtdtrb'def :
   ((mixfix_lbdtdtrb s i j) =
    (create (j - i)%Z (fun (k:Numbers.BinNums.Z) => get s (i + k)%Z))).
 
+Axiom mixfix_lbdtdtrb'spec'0 :
+  forall {a:Type} {a_WT:WhyType a},
+  forall (s:seq a) (i:Numbers.BinNums.Z) (j:Numbers.BinNums.Z),
+  (0%Z <= i)%Z /\ (i <= j)%Z /\ (j <= (length s))%Z ->
+  ((length (mixfix_lbdtdtrb s i j)) = (j - i)%Z).
+
 Axiom mixfix_lbdtdtrb'spec :
   forall {a:Type} {a_WT:WhyType a},
   forall (s:seq a) (i:Numbers.BinNums.Z) (j:Numbers.BinNums.Z),
   (0%Z <= i)%Z /\ (i <= j)%Z /\ (j <= (length s))%Z ->
-  ((length (mixfix_lbdtdtrb s i j)) = (j - i)%Z) /\
-  (forall (k:Numbers.BinNums.Z), (0%Z <= k)%Z /\ (k < (j - i)%Z)%Z ->
-   ((get (mixfix_lbdtdtrb s i j) k) = (get s (i + k)%Z))).
+  forall (k:Numbers.BinNums.Z), (0%Z <= k)%Z /\ (k < (j - i)%Z)%Z ->
+  ((get (mixfix_lbdtdtrb s i j) k) = (get s (i + k)%Z)).
 
 Parameter mixfix_lb_dtdtrb:
   forall {a:Type} {a_WT:WhyType a}, seq a -> Numbers.BinNums.Z -> seq a.
@@ -248,15 +266,22 @@ Axiom result'def3 :
 Definition infix_plpl {a:Type} {a_WT:WhyType a} (s1:seq a) (s2:seq a) : seq a :=
   let l := length s1 in create (l + (length s2))%Z (result3 s1 s2 l).
 
-Axiom infix_plpl'spec :
+Axiom infix_plpl'spec'1 :
   forall {a:Type} {a_WT:WhyType a},
   forall (s1:seq a) (s2:seq a),
-  ((length (infix_plpl s1 s2)) = ((length s1) + (length s2))%Z) /\
-  (forall (i:Numbers.BinNums.Z), (0%Z <= i)%Z /\ (i < (length s1))%Z ->
-   ((get (infix_plpl s1 s2) i) = (get s1 i))) /\
-  (forall (i:Numbers.BinNums.Z),
-   ((length s1) <= i)%Z /\ (i < (length (infix_plpl s1 s2)))%Z ->
-   ((get (infix_plpl s1 s2) i) = (get s2 (i - (length s1))%Z))).
+  ((length (infix_plpl s1 s2)) = ((length s1) + (length s2))%Z).
+
+Axiom infix_plpl'spec'0 :
+  forall {a:Type} {a_WT:WhyType a},
+  forall (s1:seq a) (s2:seq a), forall (i:Numbers.BinNums.Z),
+  (0%Z <= i)%Z /\ (i < (length s1))%Z ->
+  ((get (infix_plpl s1 s2) i) = (get s1 i)).
+
+Axiom infix_plpl'spec :
+  forall {a:Type} {a_WT:WhyType a},
+  forall (s1:seq a) (s2:seq a), forall (i:Numbers.BinNums.Z),
+  ((length s1) <= i)%Z /\ (i < (length (infix_plpl s1 s2)))%Z ->
+  ((get (infix_plpl s1 s2) i) = (get s2 (i - (length s1))%Z)).
 
 (* Why3 assumption *)
 Inductive t_unionfindmodel :=
@@ -271,148 +296,209 @@ Definition unionfindmodel_parent (self:t_unionfindmodel) : seq uint64 :=
   end.
 
 (* Why3 assumption *)
-Definition parent (self:t_unionfindmodel) (i:Numbers.BinNums.Z) :
+Inductive borrowed
+  (a:Type) :=
+  | borrowed'mk : a -> a -> Numbers.BinNums.Z -> borrowed a.
+Axiom borrowed_WhyType : forall (a:Type) {a_WT:WhyType a},
+  WhyType (borrowed a).
+Existing Instance borrowed_WhyType.
+Arguments borrowed'mk {a}.
+
+(* Why3 assumption *)
+Definition current {a:Type} {a_WT:WhyType a} (v:borrowed a) : a :=
+  match v with
+  | borrowed'mk x x1 x2 => x
+  end.
+
+(* Why3 assumption *)
+Definition final {a:Type} {a_WT:WhyType a} (v:borrowed a) : a :=
+  match v with
+  | borrowed'mk x x1 x2 => x1
+  end.
+
+(* Why3 assumption *)
+Definition id {a:Type} {a_WT:WhyType a} (v:borrowed a) : Numbers.BinNums.Z :=
+  match v with
+  | borrowed'mk x x1 x2 => x2
+  end.
+
+Parameter inherit_id:
+  Numbers.BinNums.Z -> Numbers.BinNums.Z -> Numbers.BinNums.Z.
+
+(* Why3 assumption *)
+Definition parent0 (self:t_unionfindmodel) (i:Numbers.BinNums.Z) :
     Numbers.BinNums.Z :=
   uint64'int (get (unionfindmodel_parent self) i).
 
-Parameter reach:
+Parameter reach0:
   t_unionfindmodel -> Numbers.BinNums.Z -> Numbers.BinNums.Z ->
   Numbers.BinNums.Z -> Prop.
 
-Axiom def :
+Axiom reach0_def :
   forall (self:t_unionfindmodel) (src:Numbers.BinNums.Z)
     (dst:Numbers.BinNums.Z) (len:Numbers.BinNums.Z),
-  (reach self src dst len ->
+  (reach0 self src dst len ->
    ~ (len < 0%Z)%Z /\
-   (~ (len < 0%Z)%Z ->
-    ((len = 0%Z) -> (src = dst)) /\
-    (~ (len = 0%Z) ->
-     ~ (src = dst) /\ reach self (parent self src) dst (len - 1%Z)%Z))) /\
+   ((len = 0%Z) -> (src = dst)) /\
+   (~ (len = 0%Z) ->
+    ~ (src = dst) /\ reach0 self (parent0 self src) dst (len - 1%Z)%Z)) /\
   (~ (len < 0%Z)%Z /\
    ((len = 0%Z) /\ (src = dst) \/
     ~ (len = 0%Z) /\
-    ~ (src = dst) /\ reach self (parent self src) dst (len - 1%Z)%Z) ->
-   reach self src dst len).
+    ~ (src = dst) /\ reach0 self (parent0 self src) dst (len - 1%Z)%Z) ->
+   reach0 self src dst len).
 
-Axiom reach_spec : True.
-
-(* Why3 assumption *)
-Definition in_range (self:t_unionfindmodel) (i:Numbers.BinNums.Z) : Prop :=
-  (0%Z <= i)%Z /\ (i < (length (unionfindmodel_parent self)))%Z.
-
-(* Why3 assumption *)
-Definition is_root (self:t_unionfindmodel) (i:Numbers.BinNums.Z) : Prop :=
-  in_range self i /\ ((parent self i) = i).
-
-(* Why3 assumption *)
-Definition belong (self:t_unionfindmodel) (i:Numbers.BinNums.Z)
-    (root:Numbers.BinNums.Z) : Prop :=
-  is_root self root /\ (exists len:Numbers.BinNums.Z, reach self i root len).
-
-(* Why3 assumption *)
-Definition invariant_belong (self:t_unionfindmodel) : Prop :=
-  forall (i:Numbers.BinNums.Z), in_range self i ->
-  exists root:Numbers.BinNums.Z, belong self i root.
-
-(* Why3 assumption *)
-Definition invariant_range (self:t_unionfindmodel) : Prop :=
-  forall (i:Numbers.BinNums.Z), in_range self i ->
-  in_range self (parent self i).
-
-Axiom lemma_reach_nonneg_spec :
+Axiom lemma_reach_nonneg0_spec :
   forall (self:t_unionfindmodel), forall (len:Numbers.BinNums.Z),
   forall (dst:Numbers.BinNums.Z), forall (src:Numbers.BinNums.Z),
-  reach self src dst len -> (0%Z <= len)%Z.
+  reach0 self src dst len -> (0%Z <= len)%Z.
 
-Axiom lemma_reach_iff_spec :
+Axiom lemma_reach_iff0_spec :
   forall (self:t_unionfindmodel), forall (len:Numbers.BinNums.Z),
   forall (dst:Numbers.BinNums.Z), forall (src:Numbers.BinNums.Z),
-  reach self src dst len <->
+  reach0 self src dst len <->
   (src = dst) /\ (len = 0%Z) \/
   ~ (src = dst) /\
-  (0%Z < len)%Z /\ reach self (parent self src) dst (len - 1%Z)%Z.
+  (0%Z < len)%Z /\ reach0 self (parent0 self src) dst (len - 1%Z)%Z.
 
-Axiom lemma_reach_intro_spec :
+Axiom lemma_reach_intro0_spec :
   forall (self:t_unionfindmodel),
-  (forall (src:Numbers.BinNums.Z), reach self src src 0%Z) /\
+  (forall (src:Numbers.BinNums.Z), reach0 self src src 0%Z) /\
   (forall (len:Numbers.BinNums.Z), forall (dst:Numbers.BinNums.Z),
    forall (src:Numbers.BinNums.Z), ~ (src = dst) ->
-   reach self (parent self src) dst len -> reach self src dst (len + 1%Z)%Z).
+   reach0 self (parent0 self src) dst len ->
+   reach0 self src dst (len + 1%Z)%Z).
 
 (* Why3 assumption *)
-Definition update (self:t_unionfindmodel) (i:uint64) (r:uint64) :
+Definition update0 (self:t_unionfindmodel) (i:uint64) (r:uint64) :
     t_unionfindmodel :=
   C_UnionFindModel (set (unionfindmodel_parent self) (uint64'int i) r).
 
-Axiom lemma_update_in_range_spec :
-  forall (self:t_unionfindmodel), forall (j:Numbers.BinNums.Z),
-  forall (r:uint64), forall (i:uint64), in_range self (uint64'int i) ->
-  in_range (update self i r) j <-> in_range self j.
+(* Why3 assumption *)
+Definition in_range0 (self:t_unionfindmodel) (i:Numbers.BinNums.Z) : Prop :=
+  (0%Z <= i)%Z /\ (i < (length (unionfindmodel_parent self)))%Z.
 
-Axiom lemma_update_parent_ne_spec :
+Axiom lemma_update_in_range0_spec :
   forall (self:t_unionfindmodel), forall (j:Numbers.BinNums.Z),
-  forall (r:uint64), forall (i:uint64), in_range self (uint64'int i) ->
-  in_range self j -> ~ ((uint64'int i) = j) ->
-  ((parent (update self i r) j) = (parent self j)).
+  forall (r:uint64), forall (i:uint64), in_range0 self (uint64'int i) ->
+  in_range0 (update0 self i r) j <-> in_range0 self j.
 
-Axiom lemma_update_parent_eq_spec :
+Axiom lemma_update_parent_ne0_spec :
+  forall (self:t_unionfindmodel), forall (j:Numbers.BinNums.Z),
+  forall (r:uint64), forall (i:uint64), in_range0 self (uint64'int i) ->
+  in_range0 self j -> ~ ((uint64'int i) = j) ->
+  ((parent0 (update0 self i r) j) = (parent0 self j)).
+
+Axiom lemma_update_parent_eq0_spec :
   forall (self:t_unionfindmodel), forall (r:uint64), forall (i:uint64),
-  in_range self (uint64'int i) ->
-  ((parent (update self i r) (uint64'int i)) = (uint64'int r)).
+  in_range0 self (uint64'int i) ->
+  ((parent0 (update0 self i r) (uint64'int i)) = (uint64'int r)).
 
 (* Why3 assumption *)
-Definition invariant' (self:t_unionfindmodel) : Prop :=
-  invariant_range self /\ invariant_belong self.
+Definition is_root0 (self:t_unionfindmodel) (i:Numbers.BinNums.Z) : Prop :=
+  in_range0 self i /\ ((parent0 self i) = i).
+
+(* Why3 assumption *)
+Definition belong0 (self:t_unionfindmodel) (i:Numbers.BinNums.Z)
+    (root:Numbers.BinNums.Z) : Prop :=
+  is_root0 self root /\
+  (exists len:Numbers.BinNums.Z, reach0 self i root len).
+
+(* Why3 assumption *)
+Definition invariant_belong0 (self:t_unionfindmodel) : Prop :=
+  forall (i:Numbers.BinNums.Z), in_range0 self i ->
+  exists root:Numbers.BinNums.Z, belong0 self i root.
+
+(* Why3 assumption *)
+Definition invariant_range0 (self:t_unionfindmodel) : Prop :=
+  forall (i:Numbers.BinNums.Z), in_range0 self i ->
+  in_range0 self (parent0 self i).
+
+(* Why3 assumption *)
+Definition invariant0 (self:t_unionfindmodel) : Prop :=
+  invariant_range0 self /\ invariant_belong0 self.
+
+Parameter self: t_unionfindmodel.
+
+Parameter i: uint64.
+
+Parameter r: uint64.
+
+Parameter lemma_update_belong_updated:
+  t_unionfindmodel -> uint64 -> uint64 -> Init.Datatypes.unit.
 
 (* Why3 goal *)
-Theorem lemma_update_belong_updated'vc :
-  forall (self:seq uint64) (i:uint64) (r:uint64),
-  let self1 := C_UnionFindModel self in
-  invariant' self1 /\
-  in_range self1 (uint64'int i) /\
-  in_range self1 (uint64'int r) /\ is_root self1 (uint64'int r) ->
+Theorem vc_lemma_update_belong_updated :
+  is_root0 self (uint64'int r) -> in_range0 self (uint64'int r) ->
+  in_range0 self (uint64'int i) -> invariant0 self ->
+  (forall (r1:uint64), forall (i1:uint64), in_range0 self (uint64'int i1) ->
+   ((parent0 (update0 self i1 r1) (uint64'int i1)) = (uint64'int r1))) ->
+  (forall (j:Numbers.BinNums.Z), forall (r1:uint64), forall (i1:uint64),
+   in_range0 self (uint64'int i1) -> in_range0 self j ->
+   ~ ((uint64'int i1) = j) ->
+   ((parent0 (update0 self i1 r1) j) = (parent0 self j))) ->
+  (forall (j:Numbers.BinNums.Z), forall (r1:uint64), forall (i1:uint64),
+   in_range0 self (uint64'int i1) ->
+   in_range0 (update0 self i1 r1) j <-> in_range0 self j) ->
+  (forall (src:Numbers.BinNums.Z), reach0 self src src 0%Z) /\
+  (forall (len:Numbers.BinNums.Z), forall (dst:Numbers.BinNums.Z),
+   forall (src:Numbers.BinNums.Z), ~ (src = dst) ->
+   reach0 self (parent0 self src) dst len ->
+   reach0 self src dst (len + 1%Z)%Z) ->
+  (forall (len:Numbers.BinNums.Z), forall (dst:Numbers.BinNums.Z),
+   forall (src:Numbers.BinNums.Z),
+   reach0 self src dst len <->
+   (src = dst) /\ (len = 0%Z) \/
+   ~ (src = dst) /\
+   (0%Z < len)%Z /\ reach0 self (parent0 self src) dst (len - 1%Z)%Z) ->
+  (forall (len:Numbers.BinNums.Z), forall (dst:Numbers.BinNums.Z),
+   forall (src:Numbers.BinNums.Z), reach0 self src dst len -> (0%Z <= len)%Z) ->
   forall (n:Numbers.BinNums.Z), forall (j:Numbers.BinNums.Z),
-  in_range self1 j -> reach self1 j (uint64'int i) n ->
-  belong (update self1 i r) j (uint64'int r).
+  in_range0 self j -> reach0 self j (uint64'int i) n ->
+  belong0 (update0 self i r) j (uint64'int r).
 Proof.
-intros s i' r' self (Hself_inv & Hinrange_i & Hinrange_r & Hisroot_r)
-    n j Hinrange_j Hreach.
+  (*intros h1 h2 h3 h4 h5 h6 h7 (h8,h9) h10 h11 n j h12 h13.*)
   Open Scope Z_scope.
-  pose proof (lemma_update_parent_eq_spec self r' i' Hinrange_i) as update_parent_eq.
-  pose proof (fun j p1 p2 => lemma_update_parent_ne_spec self j r' i' Hinrange_i p1 p2)
+
+  intros Hisroot_r Hinrange_r Hinrange_i Hself_inv h6 h5 h4 h3 h2 h1 n j Hinrange_j Hreach.
+  set (r' := uint64'int r).
+  set (i' := uint64'int i).
+  pose proof (lemma_update_parent_eq0_spec self r i Hinrange_i) as update_parent_eq.
+  pose proof (fun j p1 p2 => lemma_update_parent_ne0_spec self j r i Hinrange_i p1 p2)
     as update_parent_ne.
-  pose proof (fun j => lemma_update_in_range_spec self j r' i' Hinrange_i)
+  pose proof (fun j => lemma_update_in_range0_spec self j r i Hinrange_i)
     as update_in_range.
-  remember (uint64'int i') as i eqn:e; clear e.
-  remember (uint64'int r') as r eqn:e; clear e.
-  remember (update self i' r') as updated eqn:e; clear e.
+(*  remember (uint64'int i') as i eqn:e; clear e.
+  remember (uint64'int r') as r eqn:e; clear e.*)
+(*  remember (update self i' r') as updated eqn:e; clear e.*)
   
-  unfold belong.
+  unfold belong0.
   split.
-  - unfold is_root.  rewrite update_in_range. split; auto.
-    destruct (Z.eq_dec i r); try congruence.
-    rewrite update_parent_ne; auto. apply Hisroot_r.
+  - unfold is_root0.  rewrite update_in_range. split; auto.
+    destruct (Z.eq_dec i' r').
+    + unfold i', r' in *. congruence.
+    + rewrite update_parent_ne; auto. apply Hisroot_r.
   - revert j Hreach Hinrange_j.
     induction n as [n IH] using (well_founded_induction (Z.lt_wf 0));
       intros j Hreach Hinrange_j.
-    rewrite lemma_reach_iff_spec in Hreach.
+    rewrite lemma_reach_iff0_spec in Hreach.
     destruct Hreach as [[Heq Hz] | (Hne & Hpos & Hreach)].
     + rewrite Heq in *.
-      destruct (Z.eq_dec i r); [exists 0 | exists 1]; rewrite lemma_reach_iff_spec; auto.
+      destruct (Z.eq_dec i' r'); [exists 0 | exists 1]; rewrite lemma_reach_iff0_spec; auto.
       right.
-      rewrite lemma_reach_iff_spec.
+      rewrite lemma_reach_iff0_spec.
       auto with zarith.
-    + destruct (Z.eq_dec j r).
-      * exists 0.  rewrite lemma_reach_iff_spec. auto.
+    + destruct (Z.eq_dec j r').
+      * exists 0.  rewrite lemma_reach_iff0_spec. auto.
       * apply IH in Hreach; auto with zarith.
         -- destruct Hreach as [len Hreach].
            exists (len + 1).
-           rewrite lemma_reach_iff_spec.
+           rewrite lemma_reach_iff0_spec.
            right. repeat split; auto with zarith.
-           ++ apply lemma_reach_nonneg_spec in Hreach. auto with zarith.
+           ++ apply lemma_reach_nonneg0_spec in Hreach. auto with zarith.
            ++ replace (len + 1 - 1) with len; auto with zarith.
               rewrite update_parent_ne; auto.
         -- destruct Hself_inv as [Hinv_range _].
            now apply Hinv_range.
-Qed.
 
+Qed.
